@prefix irw:      <http://www.ontologydesignpatterns.org/ont/web/irw.owl#> .
@prefix rdf:      <http://www.w3.org/1999/02/22-rdf-syntax-ns#> .
@prefix rdfs:     <http://www.w3.org/2000/01/rdf-schema#> .
@prefix sp:       <http://spinrdf.org/sp#> .
@prefix spin:     <http://spinrdf.org/spin#> .
@prefix xsd:      <http://www.w3.org/2001/XMLSchema#> .

# --- Own namespaces ------------------------------------------

@prefix pc:        <http://purl.org/procurement/public-contracts#> .
@prefix pccons:    <http://purl.org/procurement/public-contracts-constraints#> . # Does not resolve (for the time being).
@prefix pcfa:      <http://purl.org/procurement/pc-filing-app#> . # Does not resolve (for the time being).

pcfa:Notice a owl:Class ;
  rdfs:subClassOf irw:InformationResource ;
  rdfs:label "Oznámení"@cs, "Notice"@en ;
  rdfs:comment "Instance této třídy reprezentuje dokument oznamující veřejnosti informace o veřejné zakázce. Veškeré údaje jsou již uvedeny přímo u veřejné zakázky. Proto instance třídy pc:Notice pouze uvádí datum svého uveřejnění a odkaz na zakázku, kde lze údaje nalézt. Je rozlišováno několik typů oznámení modelovaných různými podtřídami pc:Notice."@cs ;
  rdfs:comment "An instance of this class represents a document which notifies the public about a public contract. All data is already present in the contract itself. Therefore, the instance of pc:Notice contains only the date of publication and a link to the contract where it is possible to find all necessary information. We distinguish several types of notices which are modelled by different subclasses of pc:Notice."@en ;
  rdfs:isDefinedBy pcfa: 
  .

pcfa:ContractAwardNotice a owl:Class ;
  rdfs:subClassOf pcfa:Notice ;
  rdfs:label "Oznámení o zadání zakázky"@cs , "Contract award notice"@en ;
  rdfs:comment "Speciální typ oznámení o zakázce informující o zadání zakázky vybranému dodavateli."@cs ;
  rdfs:comment "A special type of notice which informs about awarding the contract to a chosen supplier."@en ;
  rdfs:isDefinedBy pcfa:
  .

###### pc:Contract properties

pcfa:notice a rdf:Property ;
  rdfs:label "Oznámení o zakázce"@cs, "Contract notice"@en ;
  rdfs:comment "Oznámení o zakázce publikované zadavatelem. Kardinalita 0..*"@cs ;
  rdfs:comment "Notice about a contract published by the contracting authority. Kardinalita 0..*"@en ;
  rdfs:domain pc:Contract ;
  rdfs:range pcfa:Notice ;
  rdfs:isDefinedBy pcfa:
  .

####### pcfa:Notice properties

dcterms:dateSubmitted vann:usageNote "Use for expressing the date, when a notice was submitted. The domain is pcfa:Notice."@en .

dcterms:dateAccepted vann:usageNote "Use for expressing the date, when a notice was accepted. The domain is pcfa:Notice."@en .


# pc:PriorInformationNotice
  # Mandatory data (based on TED):
    # Basic info: pc:contact, pc:contractingAuthority, pc:kind, pc:mainObject, pc:notice, pc:referenceNumber
    # Original language info: dcterms:title, pc:location, dcterms:description, pc:estimatedPrice || (pc:estimatedPriceLower && pc:estimatedPriceUpper)

# pc:ContractNotice 
  # Mandatory data (based on TED):
    # Basic info: pc:procedureType, pc:tenderDeadline
    # Original language info: pc:estimatedEndDate, pc:awardCriteriaCombination

# pc:CancellationNotice
  # Mandatory data (based on TED):
    # Cancellation date of a contract is the same as the pc:publicationDate of pc:CancellationNotice
    
### Mandatory data

pcfa:PriorInformationNotice spin:constraint pccons:TitleExists, pccons:BusinessEntityIsPublished
  . 

pccons:BusinessEntityIsPublished a sp:Construct ;
  rdfs:label "The business entity (gr:BusinessEntity) the contract references must be published."@en ;
  sp:text """
    CONSTRUCT {
      _:b0 a spin:ConstraintViolation ;
        spin:violationRoot ?contract
        .
    } WHERE {
      GRAPH <http://contracts.opendata.cz/resource/dataset/public-contracts/private> { # Insert the URI of the named graph for the private data space of the user of public contracts filing application.
        ?contract pc:contractingAuthority ?businessEntity .
      } .
      FILTER NOT EXISTS {
        GRAPH <http://ld.opendata.cz/resource/dataset/public-contracts/public> { # Insert the URI of the named graph for the public data space of the public contracts filing application
          ?businessEntity a gr:BusinessEntity .
        } .
      }
    }
  """
  .  
