@prefix c4n:      <http://vocab.deri.ie/c4n#> .
@prefix dcterms:  <http://purl.org/dc/terms/> .
@prefix foaf:     <http://xmlns.com/foaf/0.1/> .
@prefix gr:       <http://purl.org/goodrelations/v1#> .
@prefix irw:      <http://www.ontologydesignpatterns.org/ont/web/irw.owl#> .
@prefix loted:    <http://loted.eu/ontology#> .
@prefix owl:      <http://www.w3.org/2002/07/owl#> .
@prefix payment:  <http://reference.data.gov.uk/def/payment#> .
@prefix qb:       <http://purl.org/linked-data/cube#> .
@prefix rdf:      <http://www.w3.org/1999/02/22-rdf-syntax-ns#> .
@prefix rdfs:     <http://www.w3.org/2000/01/rdf-schema#> .
@prefix s:        <http://schema.org/> .
@prefix skos:     <http://www.w3.org/2004/02/skos/core#> .
@prefix vann:     <http://purl.org/vocab/vann/> .
@prefix vcard:    <http://www.w3.org/2006/vcard/ns#> .
@prefix xsd:      <http://www.w3.org/2001/XMLSchema#> .

# --- Own namespaces ------------------------------------------

@prefix pc:        <http://purl.org/procurement/public-contracts#> .
@prefix pcdt:      <http://purl.org/procurement/public-contracts-datatypes#> .

# --- Ontology metadata ---------------------------------------

pc: a owl:Ontology ;
  dcterms:title "Public Contracts Ontology"@en,
    "Ontologie pro veřejné zakázky"@cs ;
  dcterms:description "Ontologie pro veřejné zakázky poskytuje vyjadřovací prostředky pro popis zakázek zadávaných institucemi veřejné správy."@cs ;
  dcterms:description "Public Contracts Ontology offers a means of expression for describing public contracts in the public sector."@en ;
  dcterms:modified "2011-11-18"^^xsd:date ;
  vann:preferredNamespaceUri "http://purl.org/procurement/public-contracts#" ;
  vann:preferredNamespacePrefix "pc" ;
  dcterms:creator <http://purl.org/klimek#me>,
    <http://keg.vse.cz/resource/person/jindrich-mynarz>,
    <http://www.ksi.mff.cuni.cz/~necasky>,
    <http://www.facebook.com/nohis> ,
    <http://keg.vse.cz/resource/person/josef-petrak>,
    <http://keg.vse.cz/resource/person/vojtech-svatek> ;
  rdfs:seeAlso <http://code.google.com/p/public-contracts-ontology/>, <http://prefix.cc/pc> ;
  dcterms:rights <http://creativecommons.org/licenses/by/3.0/cz/> .

# --- Ontology authors  ---------------------------------------

<http://purl.org/klimek#me> a foaf:Person ;
  foaf:name "Jakub Klímek" ;
  foaf:mbox <mailto:klimek.mff@gmail.com> .
  
<http://purl.org/knap#me> a foaf:Person ;
  foaf:name "Tomáš Knap" ;
  foaf:mbox <mailto:toknap@gmail.com> .

<http://keg.vse.cz/person/jindrich-mynarz> a foaf:Person ;
  foaf:name "Jindřich Mynarz" ;
  foaf:mbox <mailto:mynarzjindrich@gmail.com> .

<http://www.ksi.mff.cuni.cz/~necasky> a foaf:Person ;
  foaf:name "Martin Nečaský" ;
  foaf:mbox <mailto:martinnec@gmail.com> .

<http://www.facebook.com/nohis> a foaf:Person ;
   foaf:name "Pavel Nohejl" ;
   foaf:mbox <mailto:nohejl.pavel@gmail.com> .
                                               
<http://keg.vse.cz/person/josef-petrak> a foaf:Person ;
  foaf:name "Josef Petrák" ;
  foaf:mbox <mailto:me@jspetrak.name> .

<http://keg.vse.cz/person/vojtech-svatek> a foaf:Person ;
  foaf:name "Vojtěch Svátek" ;
  foaf:mbox <mailto:svatek@vse.cz> .  

####### 
####### Classes
#######

# Public contract
pc:Contract a owl:Class ;
  rdfs:subClassOf c4n:Call ;
  rdfs:label "Veřejná zakázka"@cs, "Public contract"@en ;
  rdfs:comment "Základní třída pro popis veřejné zakázky"@cs ;
  rdfs:comment "Basic class for decribing a public contract"@en ;
  rdfs:isDefinedBy pc: ;
  owl:equivalentClass loted:Tender
  .

# Framework agreement
pc:FrameworkAgreement a owl:Class ;
  rdfs:subClassOf pc:Contract ;
  rdfs:label "Rámcová smlouva"@cs, "Framework agreement"@en ;
  rdfs:comment "Třída pro popis rámcové smlouvy"@cs ;
  rdfs:comment "Class for decribing a framework agreement"@en ;
  rdfs:isDefinedBy pc: 
  .

# Dynamic purchasing system
pc:DynamicPurchasingSystem a owl:Class ;
  rdfs:subClassOf pc:Contract ;
  rdfs:label "Dynamický nákupní systém"@cs, "Dynamic purchasing system"@en ;
  rdfs:comment "Třída pro popis dynamického nákupního systému"@cs ;
  rdfs:comment "Class for decribing a dynamic purchasing system"@en ;
  rdfs:isDefinedBy pc: 
  .

# Public notice
pc:Notice a owl:Class ;
  rdfs:subClassOf irw:InformationResource ;
  rdfs:label "Oznámení"@cs, "Notice"@en ;
  rdfs:isDefinedBy pc: 
  .

# Prior information notice
pc:PriorInformationNotice a owl:Class ;
  rdfs:subClassOf pc:Notice ;
  rdfs:label "Předběžné oznámení o zakázce"@cs, "Prior information notice"@en ;
  rdfs:isDefinedBy pc:
  .

# Contract notice
pc:ContractNotice a owl:Class ;
  rdfs:subClassOf pc:Notice ;
  rdfs:label "Oznámení o zakázce"@cs , "Contract notice"@en ;
  rdfs:isDefinedBy pc:
  .

# Cancellation notice
pc:CancellationNotice a owl:Class ;
  rdfs:subClassOf pc:Notice ;
  rdfs:label "Oznámení o zrušení celé veřejné zakázky"@cs , "Notice about cancellation of a whole public contract"@en ;
  rdfs:isDefinedBy pc:
  .
  
# Partial cancellation notice
pc:PartialCancellationNotice a owl:Class ;
  rdfs:subClassOf pc:Notice ;
  rdfs:label "Oznámení o zrušení částí veřejné zakázky"@cs , "Notice about cancellation of parts of a public contract"@en ;
  rdfs:isDefinedBy pc:
  .
  
# Contract notice
pc:ContractAwardNotice a owl:Class ;
  rdfs:subClassOf pc:Notice ;
  rdfs:label "Oznámení o zadání zakázky"@cs , "Contract award notice"@en ;
  rdfs:isDefinedBy pc:
  .
  
# Tender
pc:Tender a owl:Class ;
  rdfs:subClassOf gr:Offering ;
  rdfs:label "Nabídka"@cs, "Tender"@en ;
  rdfs:comment "Základní třída pro popis nabídky dodavatele"@cs ;
  rdfs:comment "Basic class for decribing a tender submitted by a supplier"@en ;
  rdfs:isDefinedBy pc:
  .
  
# Default contract award criteria type: combination of criteria (= most economically advantageous award criteria type)
pc:AwardCriteriaCombination a owl:Class ;
  owl:equivalentClass loted:AwardCriteria ;
  rdfs:label "Kombinace kritérií pro hodnocení dodaných nabídek"@cs, "Combination of contract award criteria"@en ;
  rdfs:comment "Třída pro popis kombinace kritérií pro posuzování nabídek dodavatelů"@cs ;
  rdfs:comment "Class for description of criteria combination used for tender evaluation"@en ;
  rdfs:isDefinedBy pc:
  .
 
# Contract award criteria type: lowest price
pc:AwardCriteriaLowestPrice a owl:Class ;
  rdfs:subClassOf pc:AwardCriteriaCombination ;
  rdfs:subClassOf [
	a owl:Restriction ;
    owl:onProperty pc:awardCriterion ;
    owl:maxCardinality "0"^^xsd:nonNegativeInteger
  ] ;
  rdfs:label "Nejnižší cena je jediným rozhodujícím kritériem při hodnocení dodaných nabídek"@cs, "Lowest price is the only contract award criterion"@en ;
  rdfs:comment "Třída specifikující že jediným kritériem pro posuzování nabídek dodavatelů je nejnižší cena"@cs ;
  rdfs:comment "Class specifying that the only evaluation criterion is the lowest price"@en ;
  rdfs:isDefinedBy pc: .

# Contract award criterion
pc:AwardCriterion a owl:Class ;
  rdfs:subClassOf c4n:Condition ;
  rdfs:label "Kritérium pro udělení zakázky"@cs, "Contract award criterion"@en ;
  rdfs:comment "Třída pro popis jednoho kritéria a jeho váhy."@cs ;
  rdfs:comment "Class for description of one criterion and its weight"@en ;
  rdfs:isDefinedBy pc:
  .
  
#######
####### Terminologies
#######
  
####### Concept scheme of contract procedure types

pc:ProcedureTypeScheme a skos:ConceptScheme ; 
  skos:hasTopConcept pc:Open, pc:Restricted,
    pc:Negotiated, pc:CompetitiveDialogue ;
  rdfs:comment "Schéma konceptů pro druh řízení veřejné zakázky"@cs ;
  rdfs:comment "Concept scheme for description of procedure types for public contracts"@en
  .

pc:Open a skos:Concept ;
  skos:inScheme pc:ProcedureTypeScheme ;
  rdfs:label "Otevřené"@cs, "Open"@en ;
  rdfs:comment "Otevřené řízení veřejné zakázky"@cs ;
  rdfs:comment "Open procedure type of public contract"@en ;
  rdfs:isDefinedBy pc: ;
  skos:topConceptOf pc:ProcedureTypeScheme
  .

pc:Restricted a skos:Concept ;
  skos:inScheme pc:ProcedureTypeScheme ;
  rdfs:label "Omezené"@cs, "Restricted"@en ;
  rdfs:comment "Omezené řízení veřejné zakázky"@cs ;
  rdfs:comment "Restricted procedure type of public contract"@en ;
  rdfs:isDefinedBy pc: ;
  skos:narrower pc:AcceleratedRestricted ;
  skos:topConceptOf pc:ProcedureTypeScheme
  .
  
pc:AcceleratedRestricted a skos:Concept ;
  skos:inScheme pc:ProcedureTypeScheme ;
  rdfs:label "Urychlené omezené"@cs, "Accelerated restricted"@en ;
  rdfs:comment "Urychlené omezené řízení veřejné zakázky"@cs ;
  rdfs:comment "Accelerated restricted procedure type of public contract"@en ;
  rdfs:isDefinedBy pc: ;
  skos:broader pc:Restricted
  .

pc:Negotiated a skos:Concept ;
  skos:inScheme pc:ProcedureTypeScheme ;
  rdfs:label "Vyjednávací"@cs, "Negotiated"@en ;
  rdfs:comment "Vyjednávací řízení veřejné zakázky s výzvou k účasti v soutěži"@cs ;
  rdfs:comment "Negotiated procedure type of public contract"@en ;
  rdfs:isDefinedBy pc: ;
  skos:narrower pc:AcceleratedNegotiated ;
  skos:topConceptOf pc:ProcedureTypeScheme
  .

pc:AcceleratedNegotiated a skos:Concept ;
  skos:inScheme pc:ProcedureTypeScheme ;
  rdfs:label "Urychlené vyjednávací"@cs, "Accelerated negotiated"@en ;
  rdfs:comment "Urychlené vyjednávací řízení veřejné zakázky"@cs ;
  rdfs:comment "Accelerated negotiated procedure type of public contract"@en ;
  rdfs:isDefinedBy pc: ;
  skos:broader pc:Negotiated
  .

pc:CompetitiveDialogue a skos:Concept ;
  skos:inScheme pc:ProcedureTypeScheme ;
  rdfs:label "Soutěžní dialog"@cs, "Competition dialogue"@en ;
  rdfs:comment "Soutěžní dialog jako typ řízení veřejné zakázky"@cs ;
  rdfs:comment "Competitive dialogue is the procedure type of public contract"@en ;
  rdfs:isDefinedBy pc: ;
  skos:topConceptOf pc:ProcedureTypeScheme
  .
  
####### Concept scheme of kinds of public contracts

pc:KindScheme a skos:ConceptScheme ;
  skos:hasTopConcept pc:Supplies, pc:Works, pc:Services ;
  rdfs:comment "Schéma konceptů pro druh veřejné zakázky"@cs ;
  rdfs:comment "Concept scheme for kinds of public contracts"@en
  .

pc:Supplies a skos:Concept ;
  skos:inScheme pc:KindScheme ;
  rdfs:label "Dodávky"@cs, "Supplies"@en ;
  rdfs:comment "Druhem veřejné zakázky jsou dodávky"@cs ;
  rdfs:comment "Supplies is the kind of public contract"@en ;
  rdfs:isDefinedBy pc: ;
  skos:topConceptOf pc:KindScheme
  .
  
pc:SuppliesPurchase a skos:Concept ;
  skos:broader pc:Supplies ;
  rdfs:label "Koupě"@cs, "Purchase of supplies"@en ;
  rdfs:comment "Druhem veřejné zakázky jsou dodávky formou nákupu"@cs ;
  rdfs:comment "Purchase of supplies is the kind of public contract"@en ;
  rdfs:isDefinedBy pc: ;
  .
  
pc:SuppliesLease a skos:Concept ;
  skos:broader pc:Supplies ;
  rdfs:label "Nájem"@cs, "Lease of supplies"@en ;
  rdfs:comment "Druhem veřejné zakázky jsou dodávky formou nájmu"@cs ;
  rdfs:comment "Lease of supplies is the kind of public contract"@en ;
  rdfs:isDefinedBy pc: ;
  .
  
pc:SuppliesRental a skos:Concept ;
  skos:broader pc:Supplies ;
  rdfs:label "Koupě najaté věci"@cs, "Rental of supplies"@en ;
  rdfs:comment "Druhem veřejné zakázky jsou dodávky fomou najaté věci"@cs ;
  rdfs:comment "Rental of supplies is the kind of public contract"@en ;
  rdfs:isDefinedBy pc: ;
  .
  
pc:SuppliesHire a skos:Concept ;
  skos:broader pc:Supplies ;
  rdfs:label "Koupě na splátky"@cs, "Hire of supplies"@en ;
  rdfs:comment "Druhem veřejné zakázky jsou dodávky formou koupě na splátky"@cs ;
  rdfs:comment "Hire of supplies is the kind of public contract"@en ;
  rdfs:isDefinedBy pc: ;
  .
  
pc:CombinedSupplies a skos:Concept ;
  skos:broader pc:Supplies ;
  rdfs:label "Kombinace více forem dodávek"@cs, "Combination of more kinds of supplies"@en ;
  rdfs:comment "Druhem veřejné zakázky je kombinace více forem dodávek"@cs ;
  rdfs:comment "Combination of more kinds of supplies is the kind of public contract"@en ;
  rdfs:isDefinedBy pc: ;
  .
  
pc:Works a skos:Concept ;
  skos:inScheme pc:KindScheme ;
  rdfs:label "Stavební práce"@cs, "Works"@en ;
  rdfs:comment "Druhem veřejné zakázky jsou stavební práce"@cs ;
  rdfs:comment "Works is the kind of public contract"@en ;
  rdfs:isDefinedBy pc: ;
  skos:topConceptOf pc:KindScheme
  .
  
pc:WorksExecution a skos:Concept ;
  skos:broader pc:Works ;
  rdfs:label "Provádění stavebních prací"@cs, "Execution of works"@en ;
  rdfs:comment "Druhem veřejné zakázky je provádění stavebních prací"@cs ;
  rdfs:comment "Execution of works is the kind of public contract"@en ;
  rdfs:isDefinedBy pc: ;
  .
  
pc:WorksDesignExecution a skos:Concept ;
  skos:broader pc:Works ;
  rdfs:label "Projekt a provádění stavebních prací"@cs, "Design and execution of works"@en ;
  rdfs:comment ""@cs ;
  rdfs:comment "Design and execution of works is the kind of public contract"@en ;
  rdfs:isDefinedBy pc: ;
  .
  
pc:WorksRealisation a skos:Concept ;
  skos:broader pc:Works ;
  rdfs:label ""@cs, "Realisation of works"@en ;
  rdfs:comment ""@cs ;
  rdfs:comment "Realisation, by whatever means of work, corresponding to the requirements specified by the contracting authorities"@en ;
  rdfs:isDefinedBy pc: ;
  .

pc:Services a skos:Concept ;
  skos:inScheme pc:KindScheme ;
  rdfs:label "Služby"@cs, "Services"@en ;
  rdfs:comment "Druhem veřejné zakázky jsou služby"@cs ;
  rdfs:comment "Services is the kind of public contract"@en ;
  rdfs:isDefinedBy pc: ;
  skos:topConceptOf pc:KindScheme
  .
  
pc:MaintenanceAndRepairServices a skos:Concept ;
  skos:broader pc:Services ;
  rdfs:label ""@cs, "Maintenance and repair services"@en ;
  rdfs:comment ""@cs ;
  rdfs:comment "Maintenance and repair services"@en ;
  rdfs:isDefinedBy pc: ;
  .
  
pc:LandTransportServices a skos:Concept ;
  skos:broader pc:Services ;
  rdfs:label ""@cs, "Land transport services"@en ;
  rdfs:comment ""@cs ;
  rdfs:comment "Land transport services, including armoured car services, and courier services, except transport of mail"@en ;
  rdfs:isDefinedBy pc: ;
  .
  
pc:AirTransportServices a skos:Concept ;
  skos:broader pc:Services ;
  rdfs:label ""@cs, "Air transport services"@en ;
  rdfs:comment ""@cs ;
  rdfs:comment "Air transport services of passengers and freight, except transport of mail"@en ;
  rdfs:isDefinedBy pc: ;
  .
  
pc:TransportOfMailServices a skos:Concept ;
  skos:broader pc:Services ;
  rdfs:label ""@cs, "Transport of mail by land and by air"@en ;
  rdfs:comment ""@cs ;
  rdfs:comment "Transport of mail by land and by air"@en ;
  rdfs:isDefinedBy pc: ;
  .
  
pc:TelecommunicationServices a skos:Concept ;
  skos:broader pc:Services ;
  rdfs:label ""@cs, "Telecommunications services"@en ;
  rdfs:comment ""@cs ;
  rdfs:comment "Telecommunications services"@en ;
  rdfs:isDefinedBy pc: ;
  .
  
pc:FinancialServices a skos:Concept ;
  skos:broader pc:Services ;
  rdfs:label ""@cs, "Financial services"@en ;
  rdfs:comment ""@cs ;
  rdfs:comment "Financial services: a)Insurances services b)Banking and investment services"@en ;
  rdfs:isDefinedBy pc: ;
  .
  
pc:ComputerServices a skos:Concept ;
  skos:broader pc:Services ;
  rdfs:label ""@cs, "Computer and related services"@en ;
  rdfs:comment ""@cs ;
  rdfs:comment "Computer and related services"@en ;
  rdfs:isDefinedBy pc: ;
  .
  
pc:ResearchAndDevelopmentServices a skos:Concept ;
  skos:broader pc:Services ;
  rdfs:label ""@cs, "Research and development services"@en ;
  rdfs:comment ""@cs ;
  rdfs:comment "Research and development services"@en ;
  rdfs:isDefinedBy pc: ;
  .
  
pc:AccountingServices a skos:Concept ;
  skos:broader pc:Services ;
  rdfs:label ""@cs, "Accounting, auditing and bookkeeping services"@en ;
  rdfs:comment ""@cs ;
  rdfs:comment "Accounting, auditing and bookkeeping services"@en ;
  rdfs:isDefinedBy pc: ;
  .
  
pc:MarketResearchServices a skos:Concept ;
  skos:broader pc:Services ;
  rdfs:label ""@cs, "Market research and public opinion polling services"@en ;
  rdfs:comment ""@cs ;
  rdfs:comment "Market research and public opinion polling services"@en ;
  rdfs:isDefinedBy pc: ;
  .
  
pc:ConsultingServices a skos:Concept ;
  skos:broader pc:Services ;
  rdfs:label ""@cs, "Management consulting services"@en ;
  rdfs:comment ""@cs ;
  rdfs:comment "Management consulting services and related services"@en ;
  rdfs:isDefinedBy pc: ;
  .
  
pc:ArchitecturalServices a skos:Concept ;
  skos:broader pc:Services ;
  rdfs:label ""@cs, "Architectural and engineering services"@en ;
  rdfs:comment ""@cs ;
  rdfs:comment "Architectural services; engineering services and integrated engineering services; urban planning and landscape engineering services; related scientific and technical consulting services; technical testing and analysis services"@en ;
  rdfs:isDefinedBy pc: ;
  .
  
pc:AdvertisingServices a skos:Concept ;
  skos:broader pc:Services ;
  rdfs:label ""@cs, "Advertising services"@en ;
  rdfs:comment ""@cs ;
  rdfs:comment "Advertising services"@en ;
  rdfs:isDefinedBy pc: ;
  .
  
pc:BuildingCleaningServices a skos:Concept ;
  skos:broader pc:Services ;
  rdfs:label ""@cs, "Building-cleaning services and property management services"@en ;
  rdfs:comment ""@cs ;
  rdfs:comment "Building-cleaning services and property management services"@en ;
  rdfs:isDefinedBy pc: ;
  .
  
pc:PublishingServices a skos:Concept ;
  skos:broader pc:Services ;
  rdfs:label ""@cs, "Publishing and printing services on a fee or contract basis"@en ;
  rdfs:comment ""@cs ;
  rdfs:comment "Publishing and printing services on a fee or contract basis"@en ;
  rdfs:isDefinedBy pc: ;
  .
  
pc:SewageServices a skos:Concept ;
  skos:broader pc:Services ;
  rdfs:label ""@cs, "Sewage and refuse disposal services; sanitation and similar services"@en ;
  rdfs:comment ""@cs ;
  rdfs:comment "Sewage and refuse disposal services; sanitation and similar services"@en ;
  rdfs:isDefinedBy pc: ;
  .
  
pc:HotelAndRestaurantServices a skos:Concept ;
  skos:broader pc:Services ;
  rdfs:label ""@cs, "Hotel and restaurant services"@en ;
  rdfs:comment ""@cs ;
  rdfs:comment "Hotel and restaurant services"@en ;
  rdfs:isDefinedBy pc: ;
  .
  
pc:RailTransportServices a skos:Concept ;
  skos:broader pc:Services ;
  rdfs:label ""@cs, "Rail transport services"@en ;
  rdfs:comment ""@cs ;
  rdfs:comment "Rail transport services"@en ;
  rdfs:isDefinedBy pc: ;
  .
  
pc:WaterTransportServices a skos:Concept ;
  skos:broader pc:Services ;
  rdfs:label ""@cs, "Water transport services"@en ;
  rdfs:comment ""@cs ;
  rdfs:comment "Water transport services"@en ;
  rdfs:isDefinedBy pc: ;
  .
  
pc:SupportingTransportServices a skos:Concept ;
  skos:broader pc:Services ;
  rdfs:label ""@cs, "Supporting and auxiliary transport services"@en ;
  rdfs:comment ""@cs ;
  rdfs:comment "Supporting and auxiliary transport services"@en ;
  rdfs:isDefinedBy pc: ;
  .
  
pc:LegalServices a skos:Concept ;
  skos:broader pc:Services ;
  rdfs:label ""@cs, "Legal services"@en ;
  rdfs:comment ""@cs ;
  rdfs:comment "Legal services"@en ;
  rdfs:isDefinedBy pc: ;
  .
  
pc:PersonnelPlacementServices a skos:Concept ;
  skos:broader pc:Services ;
  rdfs:label ""@cs, "Personnel placement and supply services"@en ;
  rdfs:comment ""@cs ;
  rdfs:comment "Personnel placement and supply services"@en ;
  rdfs:isDefinedBy pc: ;
  .
  
pc:InvestigationAndSecurityServices a skos:Concept ;
  skos:broader pc:Services ;
  rdfs:label ""@cs, "Investigation and security services, except armoured car services"@en ;
  rdfs:comment ""@cs ;
  rdfs:comment "Investigation and security services, except armoured car services"@en ;
  rdfs:isDefinedBy pc: ;
  .
  
pc:EducationServices a skos:Concept ;
  skos:broader pc:Services ;
  rdfs:label ""@cs, "Education and vocational education services"@en ;
  rdfs:comment ""@cs ;
  rdfs:comment "Education and vocational education services"@en ;
  rdfs:isDefinedBy pc: ;
  .
  
pc:HealthServices a skos:Concept ;
  skos:broader pc:Services ;
  rdfs:label ""@cs, "Health and social services"@en ;
  rdfs:comment ""@cs ;
  rdfs:comment "Health and social services"@en ;
  rdfs:isDefinedBy pc: ;
  .
  
pc:CulturalServices a skos:Concept ;
  skos:broader pc:Services ;
  rdfs:label ""@cs, "Recreational, cultural and sporting services"@en ;
  rdfs:comment ""@cs ;
  rdfs:comment "Recreational, cultural and sporting services"@en ;
  rdfs:isDefinedBy pc: ;
  .
  
pc:OtherServices a skos:Concept ;
  skos:broader pc:Services ;
  rdfs:label ""@cs, "Other services"@en ;
  rdfs:comment ""@cs ;
  rdfs:comment "Other services"@en ;
  rdfs:isDefinedBy pc: ;
  .
  
####### Concept scheme of types of contracting authorities

pc:AuthorityTypeScheme a skos:ConceptScheme ;
  skos:hasTopConcept pc:NationalAuthority, pc:NationalAgency, pc:LocalAuthority, pc:LocalAgency, pc:PublicBody, pc:InternationalOrganization, pc:OtherAuthority ;
  rdfs:comment "Schéma konceptů pro typy veřejných zadavatelů"@cs ;
  rdfs:comment "Concept scheme for kinds of constracting authorities"@en
  .

pc:NationalAuthority a skos:Concept ;
  skos:inScheme pc:ContractingAuthorityTypeScheme ;
  rdfs:label "Ministerstvo nebo jiný celostátní či federální orgán"@cs, "Ministry or any other national or federal authority"@en ;
  rdfs:comment "Ministerstvo nebo jiný celostátní či federální orgán včetně jejich organizačních složek"@cs ;
  rdfs:comment "Ministry or any other national or federal authority, including their regional or local sub-divisions"@en ;
  rdfs:isDefinedBy pc: ;
  skos:topConceptOf pc:AuthorityTypeScheme
  .

pc:NationalAgency a skos:Concept ;
  skos:inScheme pc:KindScheme ;
  rdfs:label "Celostátní či federální úřad/agentura"@cs, "National or federal agency/office"@en ;
  rdfs:comment "Celostátní či federální úřad/agentura"@cs ;
  rdfs:comment "National or federal agency/office"@en ;
  rdfs:isDefinedBy pc: ;
  skos:topConceptOf pc:AuthorityTypeScheme
  .

pc:LocalAuthority a skos:Concept ;
  skos:inScheme pc:KindScheme ;
  rdfs:label "Regionální či místní orgán"@cs, "Regional or local authority"@en ;
  rdfs:comment "Regionální či místní orgán"@cs ;
  rdfs:comment "Regional or local authority"@en ;
  rdfs:isDefinedBy pc: ;
  skos:topConceptOf pc:AuthorityTypeScheme
  .

pc:LocalAgency a skos:Concept ;
  skos:inScheme pc:KindScheme ;
  rdfs:label "Regionální či místní úřad/agentura"@cs, "Regional or local agency/office"@en ;
  rdfs:comment "Regionální či místní úřad/agentura"@cs ;
  rdfs:comment "Regional or local agency/office"@en ;
  rdfs:isDefinedBy pc: ;
  skos:topConceptOf pc:AuthorityTypeScheme
  .

pc:PublicBody a skos:Concept ;
  skos:inScheme pc:KindScheme ;
  rdfs:label "Veřejnoprávní instituce"@cs, "Body governed by public law"@en ;
  rdfs:comment "Veřejnoprávní instituce"@cs ;
  rdfs:comment "Body governed by public law"@en ;
  rdfs:isDefinedBy pc: ;
  skos:topConceptOf pc:AuthorityTypeScheme
  .

pc:InternationalOrganization a skos:Concept ;
  skos:inScheme pc:KindScheme ;
  rdfs:label "Evropská instituce/agentura nebo mezinárodní organizace"@cs, "European institution/agency or international organisation""@en ;
  rdfs:comment "Evropská instituce/agentura nebo mezinárodní organizace"@cs ;
  rdfs:comment "European institution/agency or international organisation"@en ;
  rdfs:isDefinedBy pc: ;
  skos:topConceptOf pc:AuthorityTypeScheme
  .

pc:OtherAuthority a skos:Concept ;
  skos:inScheme pc:KindScheme ;
  rdfs:label "Jiný typ veřejného zadavatele"@cs, "Other kind of contracting authority"@en ;
  rdfs:comment "Jiný typ veřejného zadavatele. Konkrétní hodnota zadána textově."@cs ;
  rdfs:comment "Other kind of contracting authority. Concrete value specified in text."@en ;
  rdfs:isDefinedBy pc: ;
  skos:topConceptOf pc:AuthorityTypeScheme
  .

####### Concept scheme of main activities of contracting authorities

pc:AuthorityMainActivityScheme a skos:ConceptScheme ;
  skos:hasTopConcept pc:NationalAuthority, pc:NationalAgency, pc:LocalAuthority, pc:LocalAgency, pc:PublicBody, pc:InternationalOrganization, pc:OtherAuthority ;
  rdfs:comment "Schéma konceptů pro hlavní aktivity veřejných zadavatelů"@cs ;
  rdfs:comment "Concept scheme for main activities of constracting authorities"@en
  .

pc:GeneralServicesActivity a skos:Concept ;
  skos:inScheme pc:AuthorityMainActivityScheme ;
  rdfs:label "Služby pro širokou veřejnost"@cs, "General public services"@en ;
  rdfs:comment "Služby pro širokou veřejnost"@cs ;
  rdfs:comment "General public services"@en ;
  rdfs:isDefinedBy pc: ;
  skos:topConceptOf pc:AuthorityMainActivityScheme
  .

pc:DefenceActivity a skos:Concept ;
  skos:inScheme pc:AuthorityMainActivityScheme ;
  rdfs:label "Obrana"@cs, "Defence"@en ;
  rdfs:comment "Obrana"@cs ;
  rdfs:comment "Defence"@en ;
  rdfs:isDefinedBy pc: ;
  skos:topConceptOf pc:AuthorityMainActivityScheme
  .

pc:SafetyActivity a skos:Concept ;
  skos:inScheme pc:AuthorityMainActivityScheme ;
  rdfs:label "Veřejný pořádek a bezpečnost"@cs, "Public order and safety"@en ;
  rdfs:comment "Veřejný pořádek a bezpečnost"@cs ;
  rdfs:comment "Public order and safety"@en ;
  rdfs:isDefinedBy pc: ;
  skos:topConceptOf pc:AuthorityMainActivityScheme
  .

pc:EnvironmentActivity a skos:Concept ;
  skos:inScheme pc:AuthorityMainActivityScheme ;
  rdfs:label "Životní prostředí"@cs, "Environment"@en ;
  rdfs:comment "Životní prostředí"@cs ;
  rdfs:comment "Environment"@en ;
  rdfs:isDefinedBy pc: ;
  skos:topConceptOf pc:AuthorityMainActivityScheme
  .

pc:EconomicAffairsActivity a skos:Concept ;
  skos:inScheme pc:AuthorityMainActivityScheme ;
  rdfs:label "Hospodářské a finanční záležitosti"@cs, "Economic and financial affairs"@en ;
  rdfs:comment "Hospodářské a finanční záležitosti"@cs ;
  rdfs:comment "Economic and financial affairs"@en ;
  rdfs:isDefinedBy pc: ;
  skos:topConceptOf pc:AuthorityMainActivityScheme
  .

pc:HealthActivity a skos:Concept ;
  skos:inScheme pc:AuthorityMainActivityScheme ;
  rdfs:label "Zdravotnictví"@cs, "Health"@en ;
  rdfs:comment "Zdravotnictví"@cs ;
  rdfs:comment "Health"@en ;
  rdfs:isDefinedBy pc: ;
  skos:topConceptOf pc:AuthorityMainActivityScheme
  .

pc:HousingActivity a skos:Concept ;
  skos:inScheme pc:AuthorityMainActivityScheme ;
  rdfs:label "Bydlení a občanská vybavenost"@cs, "Housing and community amenities"@en ;
  rdfs:comment "Bydlení a občanská vybavenost"@cs ;
  rdfs:comment "Housing and community amenities"@en ;
  rdfs:isDefinedBy pc: ;
  skos:topConceptOf pc:AuthorityMainActivityScheme
  .

pc:SocialProtectionActivity a skos:Concept ;
  skos:inScheme pc:AuthorityMainActivityScheme ;
  rdfs:label "Sociální služby"@cs, "Social protection"@en ;
  rdfs:comment "Sociální služby"@cs ;
  rdfs:comment "Social protection"@en ;
  rdfs:isDefinedBy pc: ;
  skos:topConceptOf pc:AuthorityMainActivityScheme
  .

pc:CulturalActivity a skos:Concept ;
  skos:inScheme pc:AuthorityMainActivityScheme ;
  rdfs:label "Rekreace, kultura a náboženství"@cs, "Recreation, culture and religion"@en ;
  rdfs:comment "Rekreace, kultura a náboženství"@cs ;
  rdfs:comment "Recreation, culture and religion"@en ;
  rdfs:isDefinedBy pc: ;
  skos:topConceptOf pc:AuthorityMainActivityScheme
  .

pc:EducationalActivity a skos:Concept ;
  skos:inScheme pc:AuthorityMainActivityScheme ;
  rdfs:label "Školství"@cs, "Education"@en ;
  rdfs:comment "Školství"@cs ;
  rdfs:comment "Education"@en ;
  rdfs:isDefinedBy pc: ;
  skos:topConceptOf pc:AuthorityMainActivityScheme
  .

pc:OtherActivity a skos:Concept ;
  skos:inScheme pc:AuthorityMainActivityScheme ;
  rdfs:label "Jiná hlavní aktivita"@cs, "Other main activity"@en ;
  rdfs:comment "Jiná hlavní aktivity veřejného zadavatele. Konkrétní hodnota zadána textově."@cs ;
  rdfs:comment "Other main activity of contracting authority. Concrete value specified in text."@en ;
  rdfs:isDefinedBy pc: ;
  skos:topConceptOf pc:AuthorityMainActivityScheme
  .

########
######## Properties
########

####### pc:Contract properties

# Contract main contact
pc:contact a owl:FunctionalProperty ;
  rdfs:label "Hlavní kontakt pro zakázku"@cs, "Main contact for a contract"@en ;
  rdfs:comment "Hlavní kontakt pro zakázku. Kardinalita 0..1"@cs ;
  rdfs:comment "Main contact for a contract. Cardinality 0..1"@en ;
  rdfs:domain pc:Contract ;
  rdfs:range vcard:VCard ;
  rdfs:isDefinedBy pc:
  .

# Kind
pc:kind a owl:FunctionalProperty, qb:CodedProperty ;
  rdfs:label "Druh zakázky"@cs, "Type of contract"@en ;
  rdfs:comment "Druh zakázky. Kardinalita 0..1"@cs ;
  rdfs:comment "Type or kind of contract. Cardinality 0..1"@en ;
  rdfs:domain pc:Contract ;
  rdfs:range skos:Concept, [
    a owl:Restriction ;
    owl:onProperty skos:inScheme ;
    owl:hasValue pc:KindScheme
  ] ;
  rdfs:isDefinedBy pc:
  .
  
# Type of procedure
pc:procedureType a owl:FunctionalProperty, qb:CodedProperty ;
  rdfs:label "Druh řízení zakázky"@cs, "Type of procedure of contract"@en ;
  rdfs:comment "Druh řízení zakázky. Kardinalita 0..1"@cs ;
  rdfs:comment "Type of procedure of contract. Cardinality 0..1"@en ;
  rdfs:domain pc:Contract ;
  rdfs:range skos:Concept, [
    a owl:Restriction ;
    owl:onProperty skos:inScheme ;
    owl:hasValue pc:ProcedureTypeScheme
  ] ;
  rdfs:isDefinedBy pc: ;
  owl:equivalentProperty loted:PR
  .

# Contracting authority
pc:contractingAuthority a owl:FunctionalProperty ;
  rdfs:subPropertyOf [
    owl:inverseOf c4n:issues
  ] ;
  rdfs:label "Zadavatel"@cs, "Contracting authority"@en ;
  rdfs:comment "Zadavatel zakázky. Kardinalita 0..1"@cs ;
  rdfs:comment "Contracting authority. Cardinality 0..1"@en ;
  rdfs:domain pc:Contract ;
  rdfs:range gr:BusinessEntity ;
  rdfs:isDefinedBy pc:
  .

# Product or service requested in the contract
pc:item a rdf:Property ;
  rdfs:subPropertyOf dcterms:hasPart ;
  rdfs:domain [
    a owl:Class ;
    owl:unionOf ( pc:Contract pc:Tender )
  ] ;
  rdfs:range gr:Offering ;
  rdfs:comment "Vlastnost pro přiřazení položky veřejné zakázce. Kardinalita 0..*"@cs ;
  rdfs:comment "Property for attachment of an Item to a public contract. Cardinality 0..*"@en ;
  rdfs:isDefinedBy pc:
  .
  
# Main object 
pc:mainObject a owl:FunctionalProperty ;
  rdfs:subPropertyOf dcterms:subject ;
  rdfs:label "Hlavní předmět zakázky"@cs, "Main object of contract"@en ;
  rdfs:comment "Vlastnost pro hlavní předmět veřejné zakázky. Kardinalita 0..1"@cs ;
  rdfs:comment "Property for main object of public contract. Cardinality 0..1"@en ;
  rdfs:domain pc:Contract ;
  rdfs:range skos:Concept ;
  rdfs:isDefinedBy pc:
  .
  
# Additional object 
pc:additionalObject a rdf:Property ;
  rdfs:subPropertyOf dcterms:subject ;
  rdfs:label "Další předmět zakázky"@cs, "Additional object of contract"@en ;
  rdfs:comment "Vlastnost pro další předmět veřejné zakázky. Kardinalita 0..*"@cs ;
  rdfs:comment "Property for additional object of public contract. Cardinality 0..*"@en ;
  rdfs:domain pc:Contract ;
  rdfs:range skos:Concept ;
  rdfs:isDefinedBy pc:
  .

# Location
pc:location a rdf:Property ;
  rdfs:label "Místo uskutečnění zakázky"@cs, "Place of contract's realization"@en ;
  rdfs:comment "Místo, kde dojde k dodání produktu nebo služby nasmlouvané ve veřejné zakázce. Kardinalita 0..*"@cs ;
  rdfs:comment "Place of delivery of contracted product or service. Cardinality 0..*"@en ;
  rdfs:domain pc:Contract ;
  rdfs:range s:Place ;
  rdfs:isDefinedBy pc:
  .
  
# On behalf of
pc:onBehalfOf a rdf:Property ;
  rdfs:label "Jménem"@cs, "On behalf of"@en ;
  rdfs:comment "Zadání zakázky jménem jiných veřejných zadavatelů. Kardinalita 0..*"@cs ;
  rdfs:comment "Contract award on behalf of other contracting authorities. Cardinality 0..*"@en ;
  rdfs:domain pc:Contract ;
  rdfs:range gr:BusinessEntity ;
  rdfs:isDefinedBy pc:
  .

# Contract notice
pc:notice a rdf:Property ;
  rdfs:label "Oznámení o zakázce"@cs, "Contract notice"@en ;
  rdfs:domain pc:Contract ;
  rdfs:range pc:Notice ;
  rdfs:isDefinedBy pc:
  .

####### ABSTRACT
# Price
pc:contractPrice a rdf:Property ;
  rdfs:label "Cena"@cs, "Price"@en ;
  rdfs:comment "Abstraktní vlastnost pro cenu veřejné zakázky"@cs ;
  rdfs:comment "Abstract property for price of public contract"@en ;
  rdfs:domain pc:Contract ;
  rdfs:range gr:PriceSpecification ;
  rdfs:isDefinedBy pc:
  .
  
# Total quantity or scope
pc:totalQuantityOrScope a owl:FunctionalProperty ;
  rdfs:label "Množství nebo rozsah zakázky"@cs, "Total quantity or scope"@en ;
  rdfs:comment "Množství nebo rozsah zakázky. Kardinalita 0..1"@cs ;
  rdfs:comment "Property for Total quantity or scope. Cardinality 0..1"@en ;
  rdfs:domain pc:Contract ;
  rdfs:range xsd:string ;
  rdfs:isDefinedBy pc:
  .

# Exact estimated contract price
pc:estimatedPrice a owl:FunctionalProperty ;
  rdfs:subPropertyOf pc:contractPrice ;
  rdfs:label "Přesná odhadovaná cena cena"@cs, "Exact estimated price"@en ;
  rdfs:comment "Vlastnost pro přesnou odhadovanou cenu veřejné zakázky. Pokud je odhadovanou cenou interval, použijte vlastnosti pc:estimatedPriceLower a pc:estimatedPriceUpper. Kardinalita 0..1"@cs ;
  rdfs:comment "Property for exact estimated price of public contract. If only estimated interval is known, use pc:estimatedPriceLower and pc:estimatedPriceUpper properties instead. Cardinality 0..1"@en ;
  rdfs:isDefinedBy pc:
  .
  
# Lower range of estimated contract price
pc:estimatedPriceLower a owl:FunctionalProperty ;
  rdfs:subPropertyOf pc:contractPrice ;
  rdfs:label "Dolní mez odhadované ceny"@cs, "Lower range of estimated price"@en ;
  rdfs:comment "Vlastnost pro dolní mez odhadované ceny veřejné zakázky. Pokud je známa přesná odhadovaná cena, použijte vlastnost pc:estimatedPrice. Kardinalita 0..1"@cs ;
  rdfs:comment "Property for lower bound of estimated price of public contract. If exact estimated price is known, use pc:estimatedPrice instead. Cardinality 0..1"@en ;
  rdfs:isDefinedBy pc:
  .
  
# Upper range of estimated contract price
pc:estimatedPriceUpper a owl:FunctionalProperty ;
  rdfs:subPropertyOf pc:contractPrice ;
  rdfs:label "Horní mez odhadované ceny"@cs, "Upper range of estimated price"@en ;
  rdfs:comment "Vlastnost pro horní mez odhadované ceny veřejné zakázky. Pokud je známa přesná odhadovaná cena, použijte vlastnost pc:estimatedPrice. Kardinalita 0..1"@cs ;
  rdfs:comment "Property for upper bound of estimated price of public contract. If exact estimated price is known, use pc:estimatedPrice instead. Cardinality 0..1"@en ;
  rdfs:isDefinedBy pc:
  .

# Exact duration of contract in days
pc:durationDays a owl:FunctionalProperty ;
  rdfs:label "Doba trvání zakázky ve dnech"@cs, "Exact duration of contract in days"@en ;
  rdfs:comment "Vlastnost pro dobu trvání zakázky ve dnech. Kardinalita 0..1"@cs ;
  rdfs:comment "Property for exact duration of contract in days. Cardinality 0..1"@en ;
  rdfs:domain pc:Contract ;
  rdfs:range xsd:positiveInteger ;
  rdfs:isDefinedBy pc:
  .
  
# Exact duration of contract in months
pc:durationMonths a owl:FunctionalProperty ;
  rdfs:label "Doba trvání zakázky v měsících"@cs, "Exact duration of contract in months"@en ;
  rdfs:comment "Vlastnost pro dobu trvání zakázky v měsících. Kardinalita 0..1"@cs ;
  rdfs:comment "Property for exact duration of contract in months. Cardinality 0..1"@en ;
  rdfs:domain pc:Contract ;
  rdfs:range xsd:positiveInteger ;
  rdfs:isDefinedBy pc:
  .
  
# Exact duration of contract in years
pc:durationYears a owl:FunctionalProperty ;
  rdfs:label "Doba trvání zakázky v letech"@cs, "Exact duration of contract in years"@en ;
  rdfs:comment "Vlastnost pro dobu trvání zakázky v letech. Kardinalita 0..1"@cs ;
  rdfs:comment "Property for exact duration of contract in years. Cardinality 0..1"@en ;
  rdfs:domain pc:Contract ;
  rdfs:range xsd:positiveInteger ;
  rdfs:isDefinedBy pc:
  .

# Time-limit for receipt of tenders or requests to participate
pc:tenderDeadline a owl:FunctionalProperty ;
  rdfs:subPropertyOf dcterms:date ;
  rdfs:label "Lhůta pro doručení nabídek nebo přijetí žádostí o účast"@cs,
    "Time-limit for receipt of tenders or requests to participate"@en ;
  rdfs:comment "Vlastnost pro lhůtu pro doručení nabídek nebo přijetí žádostí o účast. Kardinalita 0..1"@cs ;
  rdfs:comment "Property for time limit for receipt of tenders or requests to participate. Cardinality 0..1"@en ;
  rdfs:domain pc:Contract ;
  rdfs:range xsd:date ;
  rdfs:isDefinedBy pc: ;
  owl:equivalentProperty loted:DT
  .
  
# Contract publication date
pc:publicationDate a owl:FunctionalProperty ;
  rdfs:label "Datum zveřejnění zakázky"@cs, "Contract publication date"@en ;
  rdfs:comment "Vlastnost pro lhůtu pro doručení nabídek nebo přijetí žádostí o účast. Kardinalita 0..1"@cs ;
  rdfs:comment "Property for time limit for receipt of tenders or requests to participate. Cardinality 0..1"@en ;
  rdfs:domain pc:Notice ;
  rdfs:range xsd:date ;
  rdfs:subPropertyOf dcterms:issued ;
  rdfs:isDefinedBy pc: ;
  owl:equivalentProperty loted:PD
  .
  
# Date of contract award
pc:awardDate a owl:FunctionalProperty ;
  rdfs:label "Datum přidělení zakázky"@cs, "Date of contract award"@en ;
  rdfs:comment "Vlastnost pro datum přidělení zakázky dodavateli. Kardinalita 0..1"@cs ;
  rdfs:comment "Property for date of contract award to a supplier. Cardinality 0..1"@en ;
  rdfs:domain pc:Contract ;
  rdfs:range xsd:date ;
  rdfs:subPropertyOf dcterms:date ;
  rdfs:isDefinedBy pc:
  .
  
# Start date of contract
pc:startDate a owl:FunctionalProperty ;
  rdfs:label "Datum začátku realizace zakázky"@cs, "Start date of contract"@en ;
  rdfs:comment "Vlastnost pro datum začátku realizace zakázky, které je uvedené ve smlouvě. Kardinalita 0..1"@cs ;
  rdfs:comment "Property for start date of public contract realization coming from the contract's text. Cardinality 0..1"@en ;
  rdfs:domain pc:Contract ;
  rdfs:range xsd:date ;
  rdfs:subPropertyOf dcterms:date ;
  rdfs:isDefinedBy pc:
  .
  
# End date of contract
pc:estimatedEndDate a owl:FunctionalProperty ;
  rdfs:label "Očekávané datum konce realizace zakázky"@cs, "Estimated end date of contract"@en ;
  rdfs:comment "Vlastnost pro očekávané datum konce realizace zakázky. Kardinalita 0..1"@cs ;
  rdfs:comment "Property for estimated end date of public contract realization. Cardinality 0..1"@en ;
  rdfs:domain pc:Contract ;
  rdfs:range xsd:date ;
  rdfs:subPropertyOf dcterms:date ;
  rdfs:isDefinedBy pc:
  .

# Actual end date of contact's realization
pc:actualEndDate a owl:FunctionalProperty ; 
  rdfs:label "Skutečné datum konce realizace zakázky"@cs, "Actual end date of contract"@en ;
  rdfs:comment "Vlastnost pro skutečné datum konce realizace zakázky. Kardinalita 0..1"@cs ;
  rdfs:comment "Property for actual end date of public contract's realization. Cardinality 0..1"@en ;
  rdfs:domain pc:Contract ;
  rdfs:range xsd:date ;
  rdfs:subPropertyOf dcterms:date ;
  rdfs:isDefinedBy pc:
  .

# Date of cancellation
pc:cancellationDate a owl:FunctionalProperty ;
  rdfs:label "Datum zrušení zakázky"@cs, "Date when the contract was cancelled"@en ;
  rdfs:comment "Vlastnost určující datum, kdy byla zakázka zrušena. Kardinalita 0..1"@cs ;
  rdfs:comment  "Property specifying the date when the contract was cancelled. Cardinality 0..1"@en ;
  rdfs:domain pc:Contract ;
  rdfs:range xsd:date ;
  rdfs:subPropertyOf dcterms:date ;
  rdfs:isDefinedBy pc:
  .

# Combination of contract award criteria
pc:awardCriteriaCombination a owl:FunctionalProperty ;
  rdfs:label "Kombinace kritérií pro hodnocení nabídek dodavatelů zakázky."@cs, "Criteria combination for tender evaluation."@en ;
  rdfs:comment "Vlastnost pro nastavení kombinace kritérií pro hodnocení nabídek dodavatelů. Kardinalita 0..1"@cs ;
  rdfs:comment "Property for criteria combination for tender evaluation. Cardinality 0..1"@en ;
  rdfs:domain pc:Contract ;
  rdfs:range pc:AwardCriteriaCombination ;
  rdfs:isDefinedBy pc:
  .
  
# Contract award criterion
pc:awardCriterion a rdf:Property ;
  rdfs:label "Kritérium pro zadání zakázky."@cs, "Critera for contract award."@en, 
    "Critères d'attribution"@fr, "Vergabekriterien"@de ;
  rdfs:comment "Vlastnost pro nastavení jednoho kritéria pro hodnocení nabídek dodavatelů. Kardinalita 0..*"@cs ;
  rdfs:comment "Property for setting a criterion for tender evaluation. Cardinality 0..*"@en ;
  rdfs:domain pc:AwardCriteriaCombination ;
  rdfs:range pc:AwardCriterion ;
  rdfs:isDefinedBy pc: ;
  owl:equivalentProperty loted:AC
  .

# Contract file reference number
pc:referenceNumber a owl:FunctionalProperty ;
  rdfs:label "Spisové číslo zakázky"@cs, "File reference number"@en ;
  rdfs:comment "Spisové číslo zakázky přidělené veřejným zadavatelem. Kardinalita 0..1"@cs ;
  rdfs:comment "File reference number attributed by the contracting authority. Cardinality 0..1"@en ;
  rdfs:domain [
    a owl:Class ;
    owl:unionOf ( pc:Contract pc:Notice )
  ] ;
  rdfs:range xsd:string ;
  rdfs:isDefinedBy pc:
  .

# Contract lot
pc:lot a rdf:Property ;  
  rdfs:domain pc:Contract ;
  rdfs:range pc:Contract ;
  rdfs:label "Část zakázky"@cs, "Contract lot"@en ;
  rdfs:comment "Vlastnost pro specifikaci části zakázky. Zakázku rozděluje na části zadavatel, pokud je zakázka přiliš velká. Dodavatelé podávají nabídky na každou část odděleně a pro každou část zakázky je vybrán samostatný dodavatel. Pro samotnou zakázku nabídky nejsou podávány. Kardinalita 0..*"@cs ;
  rdfs:comment "Property for specifying contract lot. When contract is too big, it is split to lots by contracting authority. Suppliers then tender each lot separately. For each lot the authority awards a separate tender. The contract itself has no tenders. Cardinality 0..*"@en ;  
  rdfs:isDefinedBy pc:
  .
  
# Public contract is contracted on the base of a framework agreement
pc:frameworkAgreement a rdf:Property ;
  rdfs:domain pc:Contract ;
  rdfs:range pc:FrameworkAgreement 
  rdfs:label "Na základě rámcové smlouvy"@cs, "On the base of a framework agreement"@en ;
  rdfs:comment "Veřejná zakázka je zadána na základě rámcové smlouvy. Kardinalita 0..1"@cs ;
  rdfs:comment "Public contract is contracted on the base of a framework agreement. Cardinality 0..1"@cs ;
  rdfs:isDefinedBy pc:
  .
  
# Number of tenders received
pc:numberOfTenders a owl:FunctionalProperty ;
  rdfs:label "Počet obdržených nabídek"@cs, "Number of tenders received"@en ;
  rdfs:comment "Vlastnost pro počet obdržených nabídek. Kardinalita 0..1"@cs ;
  rdfs:comment "Property for number of tenders received. Cardinality 0..1"@en ;
  rdfs:domain pc:Contract ;
  rdfs:range xsd:nonNegativeInteger ;
  rdfs:isDefinedBy pc:
  .
  
# Tender
pc:tender a rdf:Property ;
  rdfs:label "Nabídka"@cs, "Tender"@en ;
  rdfs:comment "Vlastnost pro nabídku dodavatele. Kardinalita 0..*"@cs ;
  rdfs:comment "Property for a tender submitted by a supplier. Cardinality 0..*"@en ;
  rdfs:domain pc:Contract ;
  rdfs:range pc:Tender ;
  rdfs:isDefinedBy pc:
  .
  
# Awarded tender
pc:awardedTender a owl:FunctionalProperty ;
  rdfs:subPropertyOf pc:tender ;
  rdfs:label "Vybraná nabídka"@cs, "Awarded tender"@en ;
  rdfs:comment "Vlastnost pro vítěznou nabídku dodavatele. Kardinalita 0..1"@cs ;
  rdfs:comment "Property for awarded tender submitted by a supplier. Cardinality 0..1"@en ;
  rdfs:isDefinedBy pc:
  .
  
# Subsidy supplemented for contract
pc:subsidy a rdf:Property ;
  rdfs:label "Dotace použitá pro zakázku"@cs, "Subsidy supplemented for contract"@en ;
  rdfs:comment "Vlastnost pro dotaci použitou pro zakázku. Kardinalita 0..*"@cs ;
  rdfs:comment "Property for used tender subsidy. Cardinality 0..*"@en ;
  rdfs:domain pc:Contract ;
  rdfs:range payment:Payment ;
  rdfs:isDefinedBy pc:
  .

# Agreed price appearing in the contract
pc:agreedPrice a owl:FunctionalProperty ;
  rdfs:subPropertyOf pc:contractPrice ;
  rdfs:label "Smluvní cena"@cs, "Agreed price"@en ;
  rdfs:comment "Vlastnost pro cenu napsanou na smlouvě s dodavatelem. Kardinalita 0..1"@cs ;
  rdfs:comment "Property for a price stated on the contract with the supplier. Cardinality 0..1"@en ;
  rdfs:range gr:PriceSpecification ;
  rdfs:isDefinedBy pc:
  .
  
# Actual price after contract realization
pc:actualPrice a owl:FunctionalProperty ;
  rdfs:subPropertyOf pc:contractPrice ;
  rdfs:label "Skutečná cena po realizaci zakázky"@cs, "Actual price after contract realization"@en ;
  rdfs:comment "Vlastnost pro skutečnou cenu zaplacenou za zakázku. Kardinalita 0..1"@cs ;
  rdfs:comment "Property for actual price of the public contract. Cardinality 0..1"@en ;
  rdfs:range gr:PriceSpecification ;
  rdfs:isDefinedBy pc:
  .
  
# Contract attachment
pc:attachment a rdf:Property ;
  rdfs:label "Příloha k zakázce"@cs, "Contract attachment"@en ;
  rdfs:comment "Vlastnost pro připojení ostatních příhloh. Specifikaci připojte pomocí pc:specification, smlouvu pomocí pc:agreement. Kardinalita 0..*"@cs ;
  rdfs:comment "Property for attachment of other documents. For attachment of contract specification use pc:specification. For attachment of contract agreement use pc:agreement. Cardinality 0..*"@en ;
  rdfs:domain pc:Contract ;
  rdfs:range rdf:Resource ;
  rdfs:isDefinedBy pc:
  .
  
# Contract specification
pc:specification a rdf:Property ;
  rdfs:subPropertyOf pc:attachment ;
  rdfs:label "Specifikace zakázky"@cs, "Contract specification"@en ;
  rdfs:comment "Vlastnost pro připojení dokumentů obsahujících specifikaci veřejné zakázky. Kardinalita 0..*"@cs ;
  rdfs:comment "Property for attachment of documents containing the contract specification. Cardinality 0..*"@en ;
  rdfs:isDefinedBy pc:
  .

# Contract agreement
pc:agreement a rdf:Property ;
  rdfs:subPropertyOf pc:attachment ;
  rdfs:label "Smlouva na veřejnou zakázku"@cs, "Contract agreement"@en ;
  rdfs:comment "Vlastnost pro připojení dokumentů obsahujících smlouvy na veřejnou zakázku uzavřené mezi zadavatelem a dodavatelem. Kardinalita 0..*"@cs ;
  rdfs:comment "Property for attachment of documents containing the agreement between supplier and contractor. Cardinality 0..*"@en ;
  rdfs:isDefinedBy pc:
  .
  
####### pc:Notice properties

# Previous notice
pc:previousNotice a owl:FunctionalProperty ;
  rdfs:label "Přecházející verze oznámení o zakázce"@cs, "Previous version of the contract notice"@en ;
  rdfs:comment "Odkaz na přecházející verzi totožného oznámení o zakázce. Kardinalita 0..1"@cs ;
  rdfs:comment "Reference to previous version of the same notice. Cardinality 0..1"@en ;
  rdfs:domain pc:Notice ;
  rdfs:range pc:Notice ;
  rdfs:isDefinedBy pc:
  . 
  
####### pc:FrameworkAgreement properties

# Number of operators in a framework agreement
pc:numberOfOperators a owl:FunctionalProperty ;
  rdfs:label "Počet účastníků rámcové smlouvy"@cs, "Number of operators of framework agreement"@en ;
  rdfs:comment "Počet účastníků rámcové smlouvy. Kardinalita 0..1"@cs ;
  rdfs:comment "Number of operators of framework agreement. Cardinality 0..1"@en ;
  rdfs:domain pc:FrameworkAgreement ;
  rdfs:range xsd:positiveInteger ;
  rdfs:isDefinedBy pc:
  .
  
# Maximum number of operators in a framework agreement
pc:maxNumberOfOperators a owl:FunctionalProperty ;
  rdfs:label "Maximální počet účastníků rámcové smlouvy"@cs, "Maximum number of operators of framework agreement"@en ;
  rdfs:comment "Maximální počet účastníků rámcové smlouvy. Kardinalita 0..1"@cs ;
  rdfs:comment "Maximum number of operators of framework agreement. Cardinality 0..1"@en ;
  rdfs:domain pc:FrameworkAgreement ;
  rdfs:range xsd:positiveInteger ;
  rdfs:isDefinedBy pc:
  .

####### gr:BusinessEntity properties

# Buyer's profile
pc:buyerProfile a owl:InverseFunctionalProperty ;
  rdfs:subPropertyOf foaf:homepage ;
  rdfs:label "Profilová stránka kupujícího"@cs, "Buyers's profile website"@en ;
  rdfs:comment "Vlastnost pro profilovou stránku kupujícího. Kardinalita 0..1"@cs ;
  rdfs:comment "Property for buyer's profile. Cardinality 0..1"@en ;
  rdfs:domain gr:BusinessEntity ;
  rdfs:range rdf:Resource ;
  rdfs:isDefinedBy pc:
  .
  
# Type of authority
pc:authorityType a owl:FunctionalProperty, qb:CodedProperty ;
  rdfs:label "Typ"@cs, "Kind"@en ;
  rdfs:comment "Typ veřejného zadavatele. Kardinalita 0..1"@cs ;
  rdfs:comment "Kind of contracting authority. Cardinality 0..1"@en ;
  rdfs:domain gr:BusinessEntity ;
  rdfs:range skos:Concept, [
    a owl:Restriction ;
    owl:onProperty skos:inScheme ;
    owl:hasValue pc:AuthorityTypeScheme
  ] ;
  rdfs:isDefinedBy pc:
  .
  
# Specification of other type of authority
pc:authorityTypeText a owl:FunctionalProperty ;
  rdfs:label "Typ (textově)"@cs, "Kind (in text)"@en ;
  rdfs:comment "Typ veřejného zadavatele (textově). Kardinalita 0..1"@cs ;
  rdfs:comment "Kind of contracting authority (in text). Cardinality 0..1"@en ;
  rdfs:domain gr:BusinessEntity, [
    a owl:Restriction ;
    owl:onProperty pc:authorityType ;
    owl:hasValue pc:OtherAuthority
  ] ;
  rdfs:range xsd:string ;
  rdfs:isDefinedBy pc:
  .

# Main activity of authority
pc:mainActivity a owl:FunctionalProperty, qb:CodedProperty ;
  rdfs:label "Hlavní aktivita"@cs, "Hlavní aktivita"@en ;
  rdfs:comment "Hlavní aktivita veřejného zadavatele. Kardinalita 0..1"@cs ;
  rdfs:comment "Main activity of contracting authority. Cardinality 0..1"@en ;
  rdfs:domain gr:BusinessEntity ;
  rdfs:range skos:Concept, [
    a owl:Restriction ;
    owl:onProperty skos:inScheme ;
    owl:hasValue pc:AuthorityMainActivityScheme
  ] ;
  rdfs:isDefinedBy pc:
  .
  
# Specification of other main activity of authority in text
pc:mainActivityText a owl:FunctionalProperty ;
  rdfs:label "Hlavní aktivita (textově)"@cs, "Hlavní aktivita (in text)"@en ;
  rdfs:comment "Hlavní aktivita veřejného zadavatele (textově). Kardinalita 0..1"@cs ;
  rdfs:comment "Main activity of contracting authority (in text). Cardinality 0..1"@en ;
  rdfs:domain gr:BusinessEntity, [
    a owl:Restriction ;
    owl:onProperty pc:mainActivity ;
    owl:hasValue pc:OtherAuthority
  ] ;
  rdfs:range xsd:string ;
  rdfs:isDefinedBy pc:
  .
  
####### pc:Tender properties

# Offered price in tender
pc:offeredPrice a owl:FunctionalProperty ;
  rdfs:subPropertyOf gr:hasPriceSpecification ;
  rdfs:label "Nabídnutá cena v nabídce"@cs, "Offered price in tender"@en ;
  rdfs:comment "Vlastnost pro cenu nabídnutou dodavatelem. Kardinalita 0..1"@cs ;
  rdfs:comment "Property for price offered by a supplier. Cardinality 0..1"@en ;
  rdfs:domain pc:Tender ;
  rdfs:range gr:PriceSpecification ;  
  rdfs:isDefinedBy pc:
  .
  
# Tender supplier
pc:supplier a rdf:Property ;
 rdfs:label "Dodavatel, který podal nabídku"@cs, "Tender supplier"@en ;
 rdfs:comment "Vlastnost pro dodavatele podávajícího nabídku. Kardinalita 0..1"@cs ;
 rdfs:comment "Property for supplier submitting the tender. Cardinality 0..1"@en ;
 rdfs:domain pc:Tender ;
 rdfs:range gr:BusinessEntity ;
 rdfs:isDefinedBy pc:
 .

####### pc:AwardCriterion properties

# Contract award criterion specification
pc:criterionName a owl:FunctionalProperty ;
  rdfs:label "Specifikace kritéria pro výběr dodavatele zakázky"@cs, "Contract award criterion specification"@en ;
  rdfs:comment "Vlastnost pro specifikaci typu kritéria pro hodnocení nabídky. Kardinalita 0..1"@cs ;
  rdfs:comment "Property for criterion type for tender evaluation. Cardinality 0..1"@en ;
  rdfs:domain pc:AwardCriterion ;
  rdfs:range xsd:string ;
  rdfs:isDefinedBy pc:
  .

# Contract award criterion weight
pc:criterionWeight a owl:FunctionalProperty ;
  rdfs:label "Váha kritéria pro výběr dodavatele zakázky"@cs, "Contract award criterion weight"@en ;
  rdfs:comment "Vlastnost pro specifikaci váhy kritéria pro hodnocení nabídky. Kardinalita 0..1"@cs ;
  rdfs:comment "Property for criterion weight for tender evaluation. Cardinality 0..1"@en ;
  rdfs:domain pc:AwardCriterion ;
  rdfs:range pcdt:percentage ;
  rdfs:isDefinedBy pc:
  .
